dw/DeepWeb/Proofs/TopLevelProof.v
@@ -4,7 +4,7 @@ From DeepWeb.Spec
 
 From DeepWeb.Proofs.Vst
      Require Import verif_prog.
-  
+(*Original proof  
 Theorem prog_correct: semax_prog_ext prog server Vprog Gprog.
 Proof.
   unfold semax_prog_ext.
@@ -19,8 +19,173 @@ Proof.
   split.
   { auto. }
   admit.
-Admitted.
+Admitted.*)
 
+  Ltac prove_semax_prog :=
+ split3; [ | | split3; [ | | split]];
+ [ reflexivity || fail "duplicate identifier in prog_defs"
+ | reflexivity || fail "unaligned initializer"
+ | solve [compute; repeat f_equal; apply proof_irr] || fail "comp_specs not equal"
+ |
+ | reflexivity || fail "match_globvars failed"
+ | match goal with |- match ?A with _ => _ end =>
+      let fs := fresh "fs" in set (fs := A); hnf in fs; subst fs; cbv iota beta;
+      lazymatch goal with
+      | |- False => fail "Can't find _main in Gprog" 
+      | |- _ =>  idtac 
+      end;
+      (eexists; reflexivity) || 
+        fail "Funspec of _main is not in the proper form"
+    end
+ ];
+ repeat (apply semax_func_cons_ext_vacuous; [reflexivity | reflexivity | ]).
+
+  Lemma extract_prog_main t d p m w: prog_main (Clightdefs.mkprogram t d p m w) = m.
+  Proof. unfold Clightdefs.mkprogram. destruct (build_composite_env' t w). reflexivity. Qed.
+
+  Lemma extract_compEnv t a (H: build_composite_env t = Errors.OK a)
+    d p m w:
+    a=prog_comp_env (Clightdefs.mkprogram t d p m w).
+  Proof. unfold Clightdefs.mkprogram.
+         destruct (build_composite_env' t w). 
+         rewrite e in H. inv H. reflexivity.
+  Qed.
+
+  Lemma extract_compEnv' {T} t d p m w x q:
+    (*build_composite_env t =  Errors.OK a -> x=w ->*)
+    x=w ->
+    x = 
+  @Ctypes.prog_comp_env T
+    {|
+    prog_defs := d;
+    prog_public := p;
+    prog_main := m;
+    prog_types := t;
+    prog_comp_env := w;
+    prog_comp_env_eq := q |}.
+  Proof. intros. subst. reflexivity. Qed.
+  
+Lemma FEqual {A} t t' (x x': option A) s s':
+  t=t' -> x=x' -> s=s' ->
+  PTree.Node t x s = PTree.Node t' x' s'.
+Proof. intros; subst. trivial. Qed.
+
+Lemma FEqual' {A} t t' (x x': option A) s s' c:
+  c = PTree.Node t' x' s' -> t=t' -> x=x' -> s=s' ->
+  PTree.Node t x s = c.
+Proof. intros; subst. trivial. Qed.
+
+Theorem prog_correct: semax_prog_ext prog server Vprog Gprog.
+Proof. (*
+  split3; [ | | split3; [ | | split]].
+ + reflexivity || fail "duplicate identifier in prog_defs".
+ + reflexivity || fail "unaligned initializer".
+ +  admit. (* solve [compute; repeat f_equal; apply proof_irr] || fail "comp_specs not equal".*)
+ + do 4 (apply semax_func_cons_ext_vacuous; [reflexivity | reflexivity | ]).
+   do 4 (apply semax_func_cons_ext_vacuous; [reflexivity | reflexivity | ]).
+   do 4 (apply semax_func_cons_ext_vacuous; [reflexivity | reflexivity | ]).
+   do 4 (apply semax_func_cons_ext_vacuous; [reflexivity | reflexivity | ]).
+   do 4 (apply semax_func_cons_ext_vacuous; [reflexivity | reflexivity | ]).
+   do 4 (apply semax_func_cons_ext_vacuous; [reflexivity | reflexivity | ]).
+   do 4 (apply semax_func_cons_ext_vacuous; [reflexivity | reflexivity | ]).
+   do 4 (apply semax_func_cons_ext_vacuous; [reflexivity | reflexivity | ]).
+   do 4 (apply semax_func_cons_ext_vacuous; [reflexivity | reflexivity | ]).
+   do 4 (apply semax_func_cons_ext_vacuous; [reflexivity | reflexivity | ]).
+   do 4 (apply semax_func_cons_ext_vacuous; [reflexivity | reflexivity | ]).
+   do 4 (apply semax_func_cons_ext_vacuous; [reflexivity | reflexivity | ]).
+   apply semax_func_cons_ext_vacuous; [reflexivity | reflexivity | ].
+   apply semax_func_cons_ext_vacuous; [reflexivity | reflexivity | ].
+   apply semax_func_cons_ext_vacuous; [reflexivity | reflexivity | ].
+   Check all_funcs_correct.
+   SearchAbout semax_func semax_prog_ext.
+   apply semax_func_cons_ext_vacuous. [reflexivity | reflexivity | ].
+   do 4 (apply semax_func_cons_ext_vacuous; [reflexivity | reflexivity | ]).
+   do 4 (apply semax_func_cons_ext_vacuous; [reflexivity | reflexivity | ]).
+   do 4 (apply semax_func_cons_ext_vacuous; [reflexivity | reflexivity | ]).
+   do 4 (apply semax_func_cons_ext_vacuous; [reflexivity | reflexivity | ]).
+   
+   apply semax_func_cons_ext_vacuous; [reflexivity | reflexivity | ].
+ + reflexivity || fail "match_globvars failed".
+ + match goal with |- match ?A with _ => _ end =>
+      let fs := fresh "fs" in set (fs := A); hnf in fs; subst fs; cbv iota beta;
+      lazymatch goal with
+      | |- False => fail "Can't find _main in Gprog" 
+      | |- _ =>  idtac 
+      end;
+      (eexists; reflexivity) || 
+        fail "Funspec of _main is not in the proper form"
+    end.
+ ];
+ repeat (apply semax_func_cons_ext_vacuous; [reflexivity | reflexivity | ]).*)
+  unfold semax_prog_ext.
+  split.
+  { auto. }
+  split.
+  { reflexivity. }
+  split. 
+  { remember prog as p. destruct prog.
+    specialize (extract_compEnv _ _  prog_comp_env_eq).
+    intros. specialize (H prog_defs prog_public prog_main).
+    assert (exists w: wf_composites prog_types, True).
+    { unfold wf_composites. rewrite prog_comp_env_eq. eexists; trivial. }
+    destruct H0 as [w _]. specialize (H w).
+    unfold cenv_cs. unfold CompSpecs.
+    assert (X: Ctypes.prog_comp_env p = prog_comp_env) by (subst p; reflexivity).
+
+    rewrite X, H; clear X H Heqp.
+    apply extract_compEnv. (*compute. 
+    rewrite H.
+    remember (Ctypes.prog_comp_env p).  CompSpecs.
+    unfold cenv_cs. Locate CompSpecs.
+    assert (Ctypes.prog_comp_env p = prog_comp_env). subst p. reflexivity.
+    rewrite H0; clear H0. erewrite H. unfold Clightdefs.mkprogram.
+    simpl. remember ( build_composite_env' prog_types w ). destruct s.
+    simpl. subst p. rewrite e in   prog_comp_env_eq.
+    inv   prog_comp_env_eq. apply extract_compEnv. rewrite e; clear Heqs e.
+    f_equal. compute. f_equal. f_equal.
+    clear e Heqs. unfold prog_types. Print build_composite_env. compute. unfold Ctypes.prog_comp_env.
+    simpl. Print wf_composites.  simpl.
+    simpl in H.
+     rewrite Heqp. apply extract_compEnv'.
+     remember (Errors.OK cenv_cs) as e.
+     unfold composites.
+Locate build_composite_env. 
+     simpl. compute. Locate composites.
+     remember prog as p. destruct p. 
+    apply extract_compEnv'.
+    specialize (compute. simpl. remember (prog_comp_env prog).
+    unfold prog in Heqc. Print prog_comp_env.
+    prog_comp_env
+           (Clightdefs.mkprogram c g 
+    cbn in Heqc. Time compute.
+    Time compute in Heqc.
+    eapply FEqual'. eassumption. clear Heqc.
+    apply FEqual. trivial. reflexivity. (*20s; wrongly reported to take 0.5s, probably displaying takes majority of time*)
+    Time compute. (*instantaneous*)
+    Time compute Locate prog_comp_env. Locate cenv_cs. compute. admit. }
+  split. 
+  { apply all_funcs_correct. }
+  split.
+  { auto. }
+  remember (initial_world.find_id (prog_main prog) Gprog) as q. unfold prog in Heqq. rewrite extract_prog_main in Heqq.
+  subst q. cbv iota beta. eexists. hnf.
+(*  unfold main_pre_ext.
+  reflexivity.
+  match goal with |- match ?A with _ => _ end =>
+      let fs := fresh "fs" in set (fs := A); hnf in fs; subst fs; cbv iota beta;
+      lazymatch goal with
+      | |- False => fail "Can't find _main in Gprog" 
+      | |- _ =>  idtac 
+      end;
+      (eexists; reflexivity) || 
+        fail "Funspec of _main is not in the proper form"
+    end.
+  compute in Heqq. idtac. Print initial_world.find_id.
+  Search Clightdefs.mkprogram. prog_main. unfold prog_main in Heqq.
+  hnf.*)*)
+  admit.
+            Admitted.
+            
 Theorem swap_server_is_correct : swap_server_correct.
 Proof.
   unfold swap_server_correct.
